ntor/NTOR_nosid.ec
@@ -1,0 +1,98 @@
+require import AllCore Distr List NTOR.
+require GAKE_nosid DiffieHellman.
+
+import DH.DDH DH.G DH.GP DH.FD.
+
+
+(* ------------------------------------------------------------------------------------------ *)
+(* Modified protocol *)
+(* ------------------------------------------------------------------------------------------ *)
+type pr_st_client_mod = pkey * skey.
+type pr_st_server_mod = skey * skey option.
+
+clone import GAKE_nosid as GAKE_mod with
+  type trace <- trace,
+  type pkey <- pkey,
+  type skey <- skey,
+  type key <- key,
+  type tag <- tag,
+  type pr_st_client <- pr_st_client_mod,
+  type pr_st_server <- pr_st_server_mod,
+  op dskey <- dt,
+  op dkey <- dkey,
+  op dtag <- dtag.
+
+
+(* ------------------------------------------------------------------------------------------ *)
+(* Modified rondom oracle *)
+clone import PROM.FullRO as HRO_mod_c with
+  type in_t    <= h_input,
+  type out_t   <= tag * key,
+  op   dout _  <= dtag `*` dkey,
+  type d_in_t  <= unit,
+  type d_out_t <= bool
+proof *.
+
+module type Server_mod = {
+  proc keygen() : pkey * skey
+  proc respond_session(st: pr_st_server_mod option, pk: pkey) : (pr_st_server_mod * (pkey * tag) * key) option
+}.
+
+module type Client_mod = {
+  proc new_session(pk: pkey) : pr_st_client_mod * pkey
+  proc complete_session(st: pr_st_client_mod, m: pkey * tag) : (pr_st_client_mod * key) option
+}.
+
+(* ------------------------------------------------------------------------------------------ *)
+(* Protocol using all public values as input *)
+module NTOR_S_mod (H : RO) : Server_mod = {
+  proc keygen() : (pkey * skey) = {
+    var sk_s, pk_s;
+
+    sk_s <$ dt;
+    pk_s <- g ^ sk_s;
+
+    return (pk_s, sk_s);
+  }
+
+  proc respond_session(st : pr_st_server_mod option, m2: pkey) : (pr_st_server_mod * (pkey * tag) * key) option = {
+    var sk_b, pk_se, sk_se, sko;
+    var sk, t_B;
+    var r <- None;
+    
+    match st with 
+    | None => {}
+    | Some st => {
+        (sk_b, sko) <- st;
+        sk_se <$ dt;
+        pk_se <- g ^ sk_se;
+        (t_B, sk) <@ H.get(m2 ^ sk_se, m2 ^ sk_b, g ^ sk_b, m2, pk_se);
+        r <- Some ((sk_b, Some sk_se), (pk_se, t_B), sk);
+      }
+    end;
+    return r;
+  }
+}.
+
+module NTOR_C_mod (H : RO) : Client = {
+  proc new_session(pk) : pr_st_client_mod * pkey = {
+    var pk_ce, sk_ce;
+
+    sk_ce <$ dt;
+    pk_ce <- g ^ sk_ce;
+
+    return ((pk, sk_ce), pk_ce);
+  }
+
+  proc complete_session(st: pr_st_client_mod, m3: pkey * tag) : (pr_st_client_mod * key) option = {
+    var r <- None;
+    var pk_b, sk_ce, sk, t_A;
+
+    (pk_b, sk_ce) <- st;
+    (t_A, sk) <@ H.get(m3.`1 ^ sk_ce, pk_b ^ sk_ce, pk_b, g ^ sk_ce, m3.`1);
+    if (t_A = m3.`2) {
+      r <- Some (st, sk);
+    }
+    return r;
+  }
+}.
